Prove evaluation is an identity on closed irreducible terms
This requires proving that using an empty substitution is an identity, and the
proof must be generalized to identity substitutions. Proving this lemma revealed
the substitution bug I just fixed.

ecoop17/dot_storeless_subst_aux.v
@@ -399,3 +399,55 @@ Proof.
       eauto using steps_closed.
 Qed.
 Hint Resolve evalToSomeRes_closed.
+
+(*******************)
+(* Prove irreducible closed terms evaluate to themselves (vl_evalToSome_self).
+   We must first prove that substitution leaves them unchnaged. *)
+
+(* Define what's an identity substitution, through the required property (rather than through an inductive type). *)
+Definition vr_env_id xs := forall n, n < length xs -> index n xs = Some (VarB n).
+
+(* Allow proving vr_env_id. These lemmas could probably be the constructors for
+   an inductive characterization. *)
+Lemma nil_vr_env_id: vr_env_id [].
+Proof. unfold vr_env_id; simpl; easy. Qed.
+
+Lemma cons_vr_env_id: forall env, vr_env_id env -> vr_env_id (VarB (length env) :: env).
+Proof. unfold vr_env_id; simpl; intros; case_match; beq_nat; subst; auto. Qed.
+
+Hint Resolve nil_vr_env_id cons_vr_env_id.
+
+(* Prove that an identity substitution is also an identity when lifted to our
+   language syntax. *)
+Lemma subst_closed_id_rec:
+  (forall v i env, vr_env_id env -> forall (Hcl: vr_closed i (length env) v),
+          vr_subst_all env v = Some v) /\
+  (forall T i env, vr_env_id env -> forall (Hcl: closed i (length env) T),
+          subst_all env T = Some T) /\
+  (forall t i env, vr_env_id env -> forall (Hcl: tm_closed i (length env) t),
+          tm_subst_all env t = Some t) /\
+  (forall d i env, vr_env_id env -> forall (Hcl: dm_closed i (length env) d),
+          dm_subst_all env d = Some d) /\
+  (forall d i env, vr_env_id env -> forall (Hcl: dms_closed i (length env) d),
+          dms_subst_all env d = Some d).
+Proof.
+  apply syntax_mutind; intros; simpl; trivial;
+    inverts_closed; subst; eauto;
+      repeat
+        match goal with
+        | Hind : context [ ?f _ ?s ] |- context [ match ?f ?env ?s with _ => _ end ] =>
+          lets ->: Hind env ___; eauto
+        end.
+Qed.
+
+Lemma tm_subst_closed_id: forall t i env, tm_closed i (length env) t -> vr_env_id env -> tm_subst_all env t = Some t.
+Proof. unmut_lemma subst_closed_id_rec. Qed.
+
+Lemma tm_subst_closed_id_nil: forall t i, tm_closed i 0 t -> tm_subst_all [] t = Some t.
+Proof. eauto using tm_subst_closed_id. Qed.
+Hint Resolve tm_subst_closed_id_nil.
+
+Hint Constructors steps.
+
+Lemma vl_evalToSome_self: forall v n i, irred v -> tm_closed i 0 v -> evalToSome [] v v n 0.
+Proof. unfold evalToSome; intuition eauto. Qed.
